steel/Zeta.Steel.Verifier.fst
@@ -52,7 +52,9 @@ let thread_state_inv' (t:thread_state_t)
     exists_ (A.pts_to t.serialization_buffer)
 
 let spec_verify_epoch (tsm:M.thread_state_model)
-  = { M.verifyepoch tsm with processed_entries = Seq.snoc tsm.processed_entries (VerifyEpoch())}
+  = let tsm = M.verifyepoch tsm in
+    if tsm.failed then tsm
+    else { tsm with M.processed_entries = Seq.snoc tsm.processed_entries (VerifyEpoch())}
 
 let verify_epoch_committed_entries (tsm:M.thread_state_model)
   : Lemma (M.committed_entries (spec_verify_epoch tsm) ==
@@ -188,6 +190,12 @@ let release_lock (#log_refs: AEH.log_refs_t)
                          hv bitmaps max contribs))));
     release lock
 
+let update_bitmap_spec (bm:IArray.repr M.epoch_id AEH.tid_bitmap)
+                       (e:M.epoch_id)
+                       (tid:tid)
+  : IArray.repr M.epoch_id AEH.tid_bitmap
+  = Map.upd bm e (Seq.upd (Map.sel bm e) (U16.v tid) true)
+
 let update_bitmap (#bm:erased _)
                   (tid_bitmaps: AEH.epoch_tid_bitmaps)
                   (e:M.epoch_id)
@@ -198,7 +206,7 @@ let update_bitmap (#bm:erased _)
       IArray.perm tid_bitmaps
                   (update_if b
                              (reveal bm)
-                             (Map.upd bm e (Seq.upd (Map.sel bm e) (U16.v tid) true)))
+                             (update_bitmap_spec bm e tid))
                   Set.empty)
   = let update_tid (v:larray bool n_threads)
       : STT (larray bool n_threads)
@@ -209,11 +217,161 @@ let update_bitmap (#bm:erased _)
     in
     with_value_of_key tid_bitmaps e update_tid
 
-let update_contributions
+let update_contributions_spec
          (tsm:M.thread_state_model)
-         (contributions: G.ref AEH.epoch_hash_contributions_t)
-         (e:M.epoch_id) = ()
+         (c:AEH.epoch_hash_contributions_t)
+         (e:M.epoch_id)
+  = let c_t = AEH.thread_contribs c tsm.thread_id in
+    let contrib = Map.sel tsm.epoch_hashes e in
+    AEH.upd_thread_contribs c tsm.thread_id (Map.upd c_t e contrib)
 
+let commit_entries #o (#log_refs: AEH.log_refs_t)
+                    #max #bms
+                   (#contribs:AEH.epoch_hash_contributions_t)
+                   (#tsm:M.thread_state_model)
+                   (t:thread_state_t)
+                   (mylogref:AEH.log_ref { //this thread's contribution to the aggregate state
+                     Map.sel log_refs tsm.thread_id == mylogref /\
+                     t.thread_id == tsm.thread_id
+                   })
+  : STGhostT unit o
+     (G.pts_to mylogref half (M.committed_entries tsm) `star`
+      AEH.per_thread_invariant log_refs max bms contribs t.thread_id)
+     (fun _ ->
+       G.pts_to mylogref half (spec_verify_epoch tsm).processed_entries `star`
+       G.pts_to mylogref half (spec_verify_epoch tsm).processed_entries `star`
+       pure (AEH.per_thread_contribution_is_accurate max bms tsm.thread_id (M.committed_entries tsm) (AEH.thread_contribs contribs tsm.thread_id)))
+  =  let _entries = elim_exists () in
+     rewrite (G.pts_to (Map.sel log_refs t.thread_id) half _entries)
+             (G.pts_to mylogref half _entries);
+     G.gather #_ #_ #_ #_ #(M.committed_entries tsm) #_ mylogref;
+     G.write mylogref (spec_verify_epoch tsm).processed_entries;
+     G.share mylogref;
+     rewrite (pure _) (pure _)
+
+
+[@@__reduce__]
+let forall_threads_except (i:tid) (p:tid -> vprop) =
+     AEH.forall_threads_between 0us i p `star`
+     AEH.forall_threads_between U16.(i +^ 1us) AEH.n_threads_16 p
+
+let advance_per_thread_contribution_accurate  (bitmaps:IArray.repr M.epoch_id AEH.tid_bitmap)
+                                              (max:_)
+                                              (contribs:_)
+                                              (tsm:M.thread_state_model)
+                                              (e:M.epoch_id)
+  : Lemma
+    (requires (
+      let tsm' = spec_verify_epoch tsm in
+      AEH.per_thread_contribution_is_accurate max bitmaps tsm.thread_id (M.committed_entries tsm) (AEH.thread_contribs contribs tsm.thread_id) /\
+      tsm'.last_verified_epoch == e))
+    (ensures (
+      let tsm' = spec_verify_epoch tsm in
+      AEH.per_thread_contribution_is_accurate
+        max
+        (update_bitmap_spec bitmaps e tsm.thread_id)
+        tsm.thread_id
+        tsm'.processed_entries
+        (AEH.thread_contribs (update_contributions_spec tsm contribs e) tsm.thread_id)))
+  = let tsm0 = M.verify_model (M.init_thread_state_model tsm.thread_id) (M.committed_entries tsm) in
+    let tsm' = spec_verify_epoch tsm in
+    assume (tsm' == M.verify_model (M.init_thread_state_model tsm'.thread_id) tsm'.processed_entries); //from top-level inv
+    assume (U32.v e == U32.v tsm0.last_verified_epoch + 1); //from trace property
+    let tid = U16.v tsm.thread_id in
+    let contribs' = AEH.thread_contribs (update_contributions_spec tsm contribs e) tsm.thread_id in
+    let contribs = AEH.thread_contribs contribs tsm.thread_id in
+    let bitmaps' = update_bitmap_spec bitmaps e tsm.thread_id in
+    introduce
+      forall (eid:M.epoch_id).
+        let h_contrib = Map.sel contribs' eid in
+        let h_tsm = Map.sel tsm'.epoch_hashes eid in
+        Seq.index (Map.sel bitmaps' eid) (U16.v tsm'.thread_id) == AEH.is_epoch_verified eid tsm'.last_verified_epoch /\
+        (if AEH.is_epoch_verified eid tsm'.last_verified_epoch
+        then h_contrib == h_tsm
+        else h_contrib == M.init_epoch_hash)
+    with (let h_contrib = Map.sel contribs' eid in
+          let h_tsm = Map.sel tsm'.epoch_hashes eid in
+          if eid <> e
+          then (
+            assert (Seq.index (Map.sel bitmaps eid) tid == Seq.index (Map.sel bitmaps' eid) tid);
+            assert (U32.v eid < U32.v e ==> AEH.is_epoch_verified eid tsm'.last_verified_epoch);
+            assert (AEH.is_epoch_verified eid tsm0.last_verified_epoch == AEH.is_epoch_verified eid tsm'.last_verified_epoch);
+            assert (Seq.index (Map.sel bitmaps' eid) tid == AEH.is_epoch_verified eid tsm'.last_verified_epoch);
+            if AEH.is_epoch_verified eid tsm0.last_verified_epoch
+            then (
+              assert (Map.sel contribs eid == h_contrib);
+              assume (Map.sel tsm0.epoch_hashes eid == h_tsm); //hashes of verified epochs don't change
+              assert (h_contrib == h_tsm)
+            )
+            else (
+              assert (h_contrib == M.init_epoch_hash)
+            )
+          ))
+
+
+let restore_per_thread_invariant #o
+                                 (#log_refs: AEH.log_refs_t)
+                                 (#hashes : AEH.all_epoch_hashes)
+                                 (#tid_bitmaps : AEH.epoch_tid_bitmaps)
+                                 (#max_certified_epoch : R.ref M.epoch_id)
+                                 (#contributions: G.ref AEH.epoch_hash_contributions_t)
+                                 (#hv:_)
+                                 (#bitmaps:IArray.repr M.epoch_id AEH.tid_bitmap)
+                                 (#max:_)
+                                 (#contribs:_)
+                                 (#tsm:M.thread_state_model)
+                                 (t:thread_state_t)
+                                 (mylogref:AEH.log_ref { //this thread's contribution to the aggregate state
+                                   Map.sel log_refs tsm.thread_id == mylogref /\
+                                   t.thread_id == tsm.thread_id
+                                 })
+                                 (e:M.epoch_id {   (spec_verify_epoch tsm).last_verified_epoch == e } )
+  : STGhostT unit o
+    (G.pts_to mylogref half (spec_verify_epoch tsm).processed_entries `star`
+     pure (AEH.per_thread_contribution_is_accurate max bitmaps tsm.thread_id (M.committed_entries tsm) (AEH.thread_contribs contribs tsm.thread_id)))
+    (fun _ ->
+      AEH.per_thread_invariant log_refs max (update_bitmap_spec bitmaps e tsm.thread_id) (update_contributions_spec tsm contribs e) tsm.thread_id)
+  = elim_pure _;
+    advance_per_thread_contribution_accurate bitmaps max contribs tsm e;
+    intro_pure (AEH.per_thread_contribution_is_accurate
+                    max
+                    (update_bitmap_spec bitmaps e tsm.thread_id)
+                    tsm.thread_id
+                    (spec_verify_epoch tsm).processed_entries
+                    (AEH.thread_contribs (update_contributions_spec tsm contribs e) tsm.thread_id));
+    rewrite (G.pts_to mylogref _ _)
+            (G.pts_to (Map.sel log_refs tsm.thread_id) half (spec_verify_epoch tsm).processed_entries);
+    intro_exists (spec_verify_epoch tsm).processed_entries
+                 (fun entries ->
+                    G.pts_to (Map.sel log_refs tsm.thread_id) half entries `star`
+                    pure (AEH.per_thread_contribution_is_accurate max
+                                                                  (update_bitmap_spec bitmaps e tsm.thread_id)
+                                                                  tsm.thread_id
+                                                                  entries
+                                                                  (AEH.thread_contribs (update_contributions_spec tsm contribs e) tsm.thread_id)));
+    ()
+
+
+
+let check_overflow_add32 (x y:U32.t)
+  : Pure (option U32.t)
+    (requires True)
+    (ensures fun res ->
+        if FStar.UInt.fits (U32.v x + U32.v y) 32
+        then Some? res /\
+             Some?.v res == U32.add x y
+        else None? res)
+ = let open U64 in
+   let res = U64.(Cast.uint32_to_uint64 x +^
+                  Cast.uint32_to_uint64 y)
+   in
+   if res >^ 0xffffffffuL
+   then None
+   else (assert (U64.v res  == U32.v x + U32.v y);
+         assert (U64.v res <= pow2 32);
+         let res = Cast.uint64_to_uint32 res in
+         assert (U32.v res  == U32.v x + U32.v y);
+         Some res)
 
 let verify_epoch (#tsm:M.thread_state_model)
                  (t:thread_state_t)
@@ -236,49 +394,50 @@ let verify_epoch (#tsm:M.thread_state_model)
       G.pts_to mylogref half (update_if b
                                     (M.committed_entries tsm)
                                     (M.committed_entries (spec_verify_epoch tsm))))
-  = let c = R.read t.clock in
-    let e = M.epoch_of_timestamp c in
-    R.write t.last_verified_epoch (Some e);
-    assert_ (thread_state_inv' t (M.verifyepoch tsm));
+  = let e = R.read t.last_verified_epoch in
+    let e' = check_overflow_add32 e 1ul in
+    match e' with
+    | None ->
+      R.write t.failed true; return true
 
-    let acquired = acquire lock in
-    if not acquired
-    then (
-      rewrite (maybe_acquired _ _)
-              emp;
-      return false
-    )
-    else (
-      rewrite (maybe_acquired _ _)
-              (AEH.lock_inv log_refs hashes tid_bitmaps max_certified_epoch contributions `star` can_release lock);
-      let _hv = elim_exists () in
-      let _bitmaps = elim_exists () in
-      let _max = elim_exists () in
-      let _contribs =
-        elim_exists #_ #_
-          #(AEH.lock_inv_body log_refs hashes tid_bitmaps max_certified_epoch contributions
-                              _hv _bitmaps _max)
-          ()
-      in
-      let b0 = propagate_epoch_hash t hashes e in
-      let b1 = update_bitmap tid_bitmaps e t.thread_id in
-      if not b0 || not b1
-      then ( //propagation failed, e.g., due to overflow
-        cancel lock;
-        drop _;
+    | Some e ->
+      R.write t.last_verified_epoch e;
+      assert_ (thread_state_inv' t (M.verifyepoch tsm));
+
+      let acquired = acquire lock in
+      if not acquired
+      then (
+        rewrite (maybe_acquired _ _)
+                emp;
         return false
       )
       else (
-          let _ = AEH.take_thread t.thread_id in
-          let _entries = elim_exists () in
-          rewrite (G.pts_to (Map.sel log_refs t.thread_id) half _entries)
-                  (G.pts_to mylogref half _entries);
-          G.gather #_ #_ #_ #_ #(M.committed_entries tsm) #_ mylogref;
-          G.write mylogref (spec_verify_epoch tsm).processed_entries;
-          G.share mylogref;
-          admit__()
+        rewrite (maybe_acquired _ _)
+                (AEH.lock_inv log_refs hashes tid_bitmaps max_certified_epoch contributions `star` can_release lock);
+        let _hv = elim_exists () in
+        let _bitmaps = elim_exists () in
+        let _max = elim_exists () in
+        let _contribs =
+          elim_exists #_ #_
+            #(AEH.lock_inv_body log_refs hashes tid_bitmaps max_certified_epoch contributions
+                                _hv _bitmaps _max)
+            ()
+        in
+        let b0 = propagate_epoch_hash t hashes e in
+        let b1 = update_bitmap tid_bitmaps e t.thread_id in
+        G.write contributions (update_contributions_spec tsm _contribs e);
+        if not b0 || not b1
+        then ( //propagation failed, e.g., due to overflow
+          cancel lock;
+          drop _;
+          return false
+        )
+        else (
+             let _ = AEH.take_thread t.thread_id in
+             commit_entries t mylogref;
+             admit__()
+        )
       )
-    )
 
 let spec_parser_log  = admit()
 
@@ -295,7 +454,7 @@ let create (tid:tid)
     let store : vstore = A.alloc None (as_u32 store_size) in
     let clock = R.alloc 0uL in
     let epoch_hashes = IArray.create epoch_id_hash 64ul finalize_epoch_hash in
-    let last_verified_epoch = R.alloc (None #M.epoch_id) in
+    let last_verified_epoch = R.alloc 0ul in
     let processed_entries : G.ref (Seq.seq log_entry_base) = G.alloc Seq.empty in
     let app_results : G.ref M.app_results = G.alloc Seq.empty in
     let serialization_buffer = A.alloc 0uy 4096ul in
@@ -882,26 +1041,6 @@ let check_overflow_add (x y:U64.t)
    else if res -^ x = y then Some res
    else None
 
-
-let check_overflow_add32 (x y:U32.t)
-  : Pure (option U32.t)
-    (requires True)
-    (ensures fun res ->
-        if FStar.UInt.fits (U32.v x + U32.v y) 32
-        then Some? res /\
-             Some?.v res == U32.add x y
-        else None? res)
- = let open U64 in
-   let res = U64.(Cast.uint32_to_uint64 x +^
-                  Cast.uint32_to_uint64 y)
-   in
-   if res >^ 0xffffffffuL
-   then None
-   else (assert (U64.v res  == U32.v x + U32.v y);
-         assert (U64.v res <= pow2 32);
-         let res = Cast.uint64_to_uint32 res in
-         assert (U32.v res  == U32.v x + U32.v y);
-         Some res)
 
 let st_check_overflow_add32 (x y:U32.t)
   : ST (option U32.t)
